pcuic/theories/PCUICParallelReduction.v
@@ -335,11 +335,11 @@ Section ParallelReduction.
     pred1 Γ Γ' (tConst c u) (tConst c u)
 
   (** Proj *)
-  | pred_proj i pars narg u args0 args1 arg1 :
+  | pred_proj p u args0 args1 arg1 :
     pred1_ctx Γ Γ' ->
     All2 (pred1 Γ Γ') args0 args1 ->
-    nth_error args1 (pars + narg) = Some arg1 ->
-    pred1 Γ Γ' (tProj (i, pars, narg) (mkApps (tConstruct i 0 u) args0)) arg1
+    nth_error args1 (p.(proj_npars) + p.(proj_arg)) = Some arg1 ->
+    pred1 Γ Γ' (tProj p (mkApps (tConstruct p.(proj_ind) 0 u) args0)) arg1
 
   (** Congruences *)
   | pred_abs na M M' N N' : 
@@ -538,14 +538,14 @@ Section ParallelReduction.
           pred1_ctx Γ Γ' ->
           Pctx Γ Γ' ->
           P Γ Γ' (tConst c u) (tConst c u)) ->
-      (forall (Γ Γ' : context) (i : inductive) (pars narg : nat) (u : Instance.t)
+      (forall (Γ Γ' : context) p (u : Instance.t)
               (args0 args1 : list term) (arg1 : term),
           pred1_ctx Γ Γ' ->
           Pctx Γ Γ' ->
           All2 (pred1 Γ Γ') args0 args1 ->
           All2 (P Γ Γ') args0 args1 ->
-          nth_error args1 (pars + narg) = Some arg1 ->
-          P Γ Γ' (tProj (i, pars, narg) (mkApps (tConstruct i 0 u) args0)) arg1) ->
+          nth_error args1 (p.(proj_npars) + p.(proj_arg)) = Some arg1 ->
+          P Γ Γ' (tProj p (mkApps (tConstruct p.(proj_ind) 0 u) args0)) arg1) ->
       (forall (Γ Γ' : context) (na : aname) (M M' N N' : term),
           pred1 Γ Γ' M M' ->
           P Γ Γ' M M' -> pred1 (Γ,, vass na M) (Γ' ,, vass na M') N N' ->
